Our goal is to minimize the functional \( \tilde{L}(P)\) such that:
\[  \min_{P\in D} \tilde{L}(P)                    \]
where:
\[ \tilde{L}(P) = L(P) + F(P) + G(P)\]

in which \(L(P) \) represents the total length of trajectories, \( F(P) \) represents the total force between each robot, and \( G(P) \) represents the total force between each robot and each obstacle.  To determine the appropriate space \( D \), we evaluate the Gateaux Derivative of \( \tilde{L}(P) \).

The Gateaux derivative of \( \delta \tilde{L}(P;V)\) is
\[ \delta \tilde{L}(P;V) = \delta L(P;V) + \delta F(P;V) + \delta G(P;V)\]
where \( V = (v_1,...,v_n) \) and \( v_j = (u_j,w_j) \).

We will compute the Gateaux derivatives \(\delta L(P;V) , \delta F(P;V) , \delta G(P;V)\) separately.

\subsection{The Gateaux Derivative of \( L(P) \)}
\begin{prop}
   The Gateaux Derivative of \( L(P) \) is 
\begin{align*}
    \delta L(P;v) &= \int_{0}^{1} \tilde{P'} \cdot V' \ dt.
\end{align*}

where \[ \tilde{P'} = \bigg( \frac{P'_1}{|P'_1|},\frac{P'_2}{|P'_2|}, ... , \frac{P'_N}{|P'_N|}  \bigg) .\]
\end{prop}
\begin{proof}
Expand \( L(P)  \) to get 
\[  L(P) = \int_{ 0 }^{ 1 } | P'(t)  |  \ dt = \int_{ 0 }^{ 1 } \sum_{ j=1 }^{ N }| P'_{j}(t) |  \ dt. \]
Define \( g(\varepsilon) = L(P + \epsilon V)  \). We can write \( g(\epsilon ) \) as  
\begin{align*}
    g(\varepsilon) &= \int_{ 0 }^{ 1 } \sum_{ j=1 }^{ N } | P'_{j}(t) + \epsilon V'_{j} |  \ dt \\
                   &= \int_{ 0 }^{ 1 }  \sum_{ j=1 }^{ N } \sqrt{ (x'_{j} + \epsilon u'_{j})^{2} + (y'_{2} + \epsilon w'_{j})^{2}  }  \ dt.
\end{align*}
Computing \( g'(\epsilon ) \), then gives us
\begin{align*}
   g'(\epsilon ) &= \frac{ d }{ d \epsilon  }  \int_{ 0 }^{ 1 } \sum_{ j=1 }^{ N } \sqrt{ (x'_{j } + \epsilon u'_{j})^{2} + (y'_{j} + \epsilon w'_{j})^{2} }  \ dt \\
                 &= \int_{ 0 }^{ 1 } \sum_{ j=1 }^{ N } \frac{\partial  }{\partial \epsilon  } \sqrt{ (x'_{j} + \epsilon  u'_{j})^{2} + (y'_{j} + \epsilon  w'_{j })^{2}  }  \ dt \\
                 &= \int_{ 0 }^{ 1 } \sum_{ j=1 }^{ N } \frac{ (x'_{j} + \epsilon u'_{j} ) u'_{j} + (y'_{j} + \epsilon  w'_{j}) w'_{j}  }{  \sqrt{  (x'_{j} + \epsilon  u'_{j})^{2} + (y'_{j} + \epsilon  w'_{j })^{2}  }   }  \ dt. 
\end{align*}
Taking the limit as \( \epsilon  \to 0  \), then gives us

\begin{align*}
    g'(0) &= \int_{ 0 }^{ 1 } \sum_{ j=1 }^{ N } \frac{ x'_{j} u'_{j} + y'_{j} w'_{j }  }{ \sqrt{ (x'_{j })^{2} + (y'_{j })^{2} }  }  \ dt \\
          &=  \int_{ 0 }^{ 1 }  \sum_{ j=1 }^{ N } \frac{ P'_{j} V'_{j}  }{ | P'_{j }  |  }  \ dt
\end{align*}
where \( x'_{j} u'_{j } + y'_{j } w'_{j } - P'_{j } \cdot V'_{j }  \) and \( | P'_{j } | = \sqrt{ (x'_{j })^{2} + (y'_{j})^{2}  }  \). Hence, applying the Gateaux Derivative to the total length of all possible trajectories is
\begin{align*}
    \delta L(P;v) &= \int_{0}^{1} \tilde{P'} \cdot V' \ dt.
\end{align*}

where \[ \tilde{P'} = \bigg( \frac{P'_1}{|P'_1|},\frac{P'_2}{|P'_2|}, ... , \frac{P'_N}{|P'_N|}  \bigg) .\]
\end{proof}


\subsection{The Gateaux Derivative of F(P)}

\begin{prop}
    The Gateaux Derivative of the total force between each robot is
    \[  \delta F(P;V) = \int_{0}^{1} \sum_{i=2}^{N} \sum_{j=1}^{i-1} \frac{2(P_i - P_j) \cdot (v_i - v_j)}{| P_i - P_j|^4} \ dt. \]
\end{prop}

\begin{proof}
First we expand \( F(p)  \) to get
\begin{align*}
    F(P) &= \frac{ 1 }{ 2 }  \int_{ 0 }^{ 1 } \sum_{ i,j = 1  }^{ N } F_{ij} \ dt \\
         &= \int_{ 0 }^{ 1 } \sum_{ i=2 }^{ N } \sum_{ j=1 }^{ i-1 } F_{ij} \ dt \\
         &= \int_{ 0 }^{ 1 } \sum_{ i=2 }^{ N } \sum_{ j=1 }^{ i-1 } \frac{ dt }{ | P_{i}(t) - P_{j }(t) |^{2}  }.
\end{align*}
Define \( g(\epsilon ) = F(P+\epsilon V)  \), we compute 
\begin{align*}
    g(\epsilon )&= \int_{ 0 }^{ 1 } \sum_{ i=2 }^{ N }\sum_{ j=1 }^{ i-1 } \frac{ dt }{ | (P_{i} + \epsilon v_{i} ) - (P_{j } + \epsilon v_{j }) | ^{2} } \\
                &= \int_{ 0 }^{ 1 } \sum_{ i=2 }^{ N } \sum_{ j=1 }^{ i-1 } \frac{ dt }{ [(x_{i} + \epsilon v_{i}) - (x_{j } + \epsilon u_{j} )]^{2} + [(y_{i} + \epsilon w_{i} ) - (y_{j} + \epsilon w_{j})]^{2}}   \\
                &= \int_{ 0 }^{ 1 } \sum_{ i=2 }^{ N } \sum_{ j=1 }^{ i-1 } \frac{ dt }{ [(x_{i} - x_{j }) + \epsilon (u_{i} - u_{j })]^{2} + [(y_{i} - y_{j}) + \epsilon (w_{i} - w_{j})]^{2}  }. \\
\end{align*}
We can take the derivative with respect to \( \epsilon  \) in the integrand will give us the following expression
\begin{align*}
    g'(\epsilon )&= \frac{ d }{ d \epsilon  }  \int_{ 0 }^{ 1 }  \sum_{ i=2 }^{ N } \sum_{ j=1 }^{ i-1 } \frac{ dt }{ [(x_{i} - x_{j}  ) + \epsilon (u_{i} - u_{j} )]^{2} + [(y_{i} - y_{j} ) + \epsilon (w_{i} - w_{j})]^{2} } \\
                 &= \int_{ 0 }^{ 1 } \sum_{ i=2 }^{ N } \sum_{ j=1 }^{ i-1 }    
    \frac{\partial  }{\partial \epsilon  }  \Bigg[ \frac{ 1 }{ [(x_{i } - x_{j}) + \epsilon (u_{i} - u_{j})]^{2} + [(y_{i} - y_{j}) + \epsilon (w_{i} - w_{j})]^{2} } \Bigg]  \ dt \\
                 &= \int_{ 0 }^{ 1 } \sum_{ i=2 }^{ N } \sum_{ j=1 }^{ i-1 } \frac{ 2[(x_{i} - x_{j}) + \epsilon (u_{i} - u_{j})](u_{i} - u_{j}) + 2[(y_{i} - y_{j}) + \epsilon (w_{i} - w_{j})](w_{i} - w_{j}) }{  \Big[ [(x_{i} - x_{j}) + \epsilon (u_{i} - u_{j})]^{2} + [(y_{i} - y_{j}) + \epsilon (w_{i} - w_{j})]^{2} \Big]^{2} }  \ dt.
\end{align*}
Letting \( \epsilon \to 0  \) and recalling that \( v_{i} = (u_{i}, w_{i} )  \) and \( v_{j} = (u_{j} , w_{j} ) \), we have that
\begin{align*}
    \lim_{ \epsilon  \to 0 } g'(\epsilon ) &= \int_{ 0 }^{ 1 } \sum_{ i=2 }^{ N } \sum_{ j=1 }^{ i-1 } \frac{ 2(x_{i} - x_{j})(u_{i} - u_{j}) + 2(y_{i} - y_{j})(w_{i} - w_{j}) }{ [(x_{i} - x_{j})^{2} + (y_{i} - y_{j})^{2}]^{2} }  \ dt  \\
                                           &= \int_{ 0 }^{ 1 } \sum_{ i=2 }^{ N } \sum_{ j=1 }^{ i-1 } \frac{ 2(P_{i} - P_{j}) \cdot (v_{i} - v_{j}) }{ | P_{i} - P_{j} |^{4} }  \ dt.
\end{align*}
\end{proof}
Hence, the Gateaux Derivative of the total force \( F(p) \) is 
\[  \delta F(P; V) = \int_{ 0 }^{ 1 }  \sum_{ i=2 }^{ N } \sum_{ j=1 }^{ i-1 } \frac{ 2(P_{i} - P_{j}) \cdot (v_{i} - v_{j}) }{ | P_{i} - P_{j} |^{4} }  \ dt. \]

\subsection{Gateaux Derivative of \( G(P) \)}

\begin{prop}
    Show that the Gateaux Derivative of \( G(P) \) is 
    \[  \delta G(P;v) = \int_{ 0 }^{ 1 } \sum_{ i=1 }^{ N } \sum_{ \ell = 1  }^{ M  } \frac{ -2 (P_{i} - C_{\ell} \cdot V_{i} ) }{ | r_{i \ell} |^{3} | P_{i}(t) - C_{\ell} |  }  \ dt. \]
\end{prop}
\begin{proof}
Expanding \( G(P) \), we get
\begin{align*} 
    G(P) &= \int_{0}^{1} \sum_{i=1}^{N}\sum_{\ell=1}^{M} \frac{dt}{|r_{i\ell}(t)|^2}  \\
         &= \int_{0}^{1} \sum_{i=1}^{N}\sum_{\ell=1}^{M} \frac{dt}{(\sqrt{(x_i(t) - a_{\ell})^2 + (y_i(t) - b_{\ell})^2} - R)^2}.
\end{align*}
Define \( g(\epsilon ) = G(P + \epsilon  V)  \) and write
\begin{align*}
    g(\epsilon ) &= \int_{0}^{1} \sum_{i=1}^{N}\sum_{\ell=1}^{M} \frac{dt}{(\sqrt{((x_i + \epsilon  u_i)- a_{\ell})^2 + ((y_i + \epsilon  w_i) - b_{\ell})^2} - R)^2}. \\
\end{align*}
with the Gateaux derivative being
\begin{align*}
    g'(\epsilon ) &= \int_{0}^{1}\sum_{i=1}^{N}\sum_{\ell=1}^{M} \Bigg[ -2\frac{ 2((x_i + \epsilon  u_i) - a_{\ell})u_i + 2((y_i + \epsilon  w_i) - b_{\ell})w_i}{|r_{i\ell}(t)|^3 2\sqrt{((x_i + \epsilon  u_i)- a_{\ell})^2 + ((y_i + \epsilon  w_i) - b_{\ell})^2}}  \Bigg] \ dt. \\ 
\end{align*}
Letting \( \epsilon \to 0  \), we can write
\begin{align*}
    \lim_{ \epsilon  \to 0 }  g'(\epsilon )&= \int_{ 0 }^{ 1 }  \sum_{ i=1 }^{ N } \sum_{ \ell = 1  }^{ M  } \frac{ -2[(x_{i} - a_{\ell})u_{i} + (y_{i} - b_{\ell})w_{i}] }{ | r_{i\ell} |^{3} | P_{i}(t) - C_{\ell} |  }  \ dt \\
                                           &= \int_{ 0 }^{ 1 }  \sum_{ i=1 }^{ N } \sum_{ \ell = 1  }^{ M  } \frac{ -2 (P_{i} - C_{\ell})\cdot V_{i}  }{  | r_{i \ell} | ^{3} | P_{i}(t) - C_{\ell} |  }  \ dt.
\end{align*}
Hence, we have
\[  \delta G(P;V) = \int_{ 0 }^{ 1 }  \sum_{ i=1 }^{ N } \sum_{ \ell = 1  }^{ M  } \frac{ -2 (P_{i} - C_{\ell}) \cdot V_{i}  }{  | r_{i\ell} |^{3} | P_{i}(t) - C_{\ell} |  }  \ dt. \]
\end{proof}

\subsection{Result}

Putting everything together, we end up with 
\begin{align*}
    \delta \tilde{L(P; V)} &= \delta L(P;V) +  \delta F(P;V) + \delta  G(P;V) \\
                           &= \int_{0}^{1} \bigg[ \sum_{j=1}^{N} \frac{P'_j \cdot V'_j}{|P'_j|} +\sum_{i=2}^{N} \sum_{j=1}^{i-1} \frac{2(P_i - P_j) \cdot (V_i - V_j)}{| P_i - P_j|^4} 
               - \sum_{i=1}^{N}\sum_{\ell=1}^{M} \frac{2(P_i - C_{\ell}) \cdot V_i}{\big| r_{i\ell}\big|^3\big|P_i(t) - C_l \big| } \bigg] \ dt.
\end{align*}



